\subsection{One-shot attack}

\begin{lemma}[Compression attack]

Let $\textrm{Com}$ be a compression function, $\textrm{Enc}$ be a strictly length-monotonic
encryption function, $f$ be a rendering function and $Q$ be a plaintext
predicate detectable with non-negligible advantage $\alpha$ over plaintext
distribution $\mathcal{M}$.

Then:
\begin{align*}
    \exists \alpha \text{ non-negl}:
    \forall \textrm{Enc}:
    \exists g:\\
    \exists PPT \mathcal{A}:
    \forall PPT \mathcal{S}:\\
    \text{Adv}_{\mathcal{SE}(\textrm{Enc}, \textrm{Com}), \mathcal{A}, \mathcal{S}}
    (\lambda, f, \mathcal{M}, g) = \alpha(\lambda)
\end{align*}

\end{lemma}

For a full proof, see Appendix A.

\subsection{Amplified attack}\label{subsec:amplification}

We can now amplify the attack to achieve a better probability of success by a small modification in our adversary.
The amplification is parameterized by an odd parameter $k$.

Let the amplification adversary be defined as follows:

\begin{lstlisting}[texcl,mathescape,basicstyle=\small]
def $\mathcal{A}(Q, \mathcal{M})$:
    $(r_1, r_2) \leftarrow \mathcal{O}_R(\textrm{Com}, f, Q, \mathcal{M})$

    $low = 0$
    $high = 0$

    for $i$ = $0$ to $k$:
        $l_1 = |\text{Reflect}^{\mathcal{E}_{pk}}_s(r_1)|$
        $l_2 = |\text{Reflect}^{\mathcal{E}_{pk}}_s(r_2)|$

        if $l_1 < l_2$:
            $low = low + 1$
        else:
            $high = high + 1$

    if $low > high$:
        return True
    else:
        return False
\end{lstlisting}

\begin{lemma}[Amplification]

Under the assumptions of the Compression Attack Theorem against $f, \textrm{Com}$
and compression-detectable predicate $Q$ with non-negligible
detectability margin $\alpha(\lambda)$,
the amplified adversary achieves an arbitrarily large advantage
against a non-negligible subset of elements, the
\textit{amplifiable elements} distinguished by predicate $Amp$.
\begin{align*}
    \forall \textrm{Enc}:
    \exists g:\\
    \exists PPT \mathcal{A}:
    \forall PPT \mathcal{S}:\\
    \exists Amp:
    \exists B \text{ non-negl}:
    \exists C \text{ negl}:\\
    \Pr_{s \leftarrow \mathcal{M}}[Amp(s)] = B(\lambda) \land\\
    \text{Adv}_{\mathcal{SE}(\textrm{Enc}, \textrm{Com}), \mathcal{A}, \mathcal{S}_{Amp}}
    (\lambda, f, \mathcal{M}, g) = 1 - \pi - C(k)
\end{align*}

\end{lemma}

The complete proof can be found in Appendix A.
